\hypertarget{Exercice_1}{
\Huge{\begin{center}Exercice 1\end{center} \leavevmode\newline }}

\hypertarget{resolution}{%
\LARGE{RÃ©solution}\label{resolution}}
\newline
\newline
Nous savons que:
\newline
\newline
$A \Delta B = (A \bigcap \overline{B}) \bigcup (\overline{A} \bigcap B)$
\newline
\newline
Si $A = \varnothing$ nous avons:
\newline
\newline
$A = \varnothing \Rightarrow (A \bigcup \overline{B}) = \varnothing$
\newline
$A = \varnothing \Rightarrow (\overline{A} \bigcap B) = (E \bigcup B) = B$
\newline
$A \Delta B = (A \bigcap \overline{B}) \bigcup (\overline{A} \bigcap B) = \varnothing \bigcup B = B$
